{
 "cells": [
  {
   "cell_type": "markdown",
   "metadata": {},
   "source": [
    "<hr>\n",
    "\n",
    "# Assigment: Recurrence Relation\n",
    "\n",
    "**Author:** *Ritesh Mandal*\n",
    "\n",
    "**Submission Date:** \n",
    "\n",
    "**Module:** Data Structure and Algorithms\n",
    "\n",
    "**Instructor:** Priya Bhatia\n",
    "\n",
    "<hr>"
   ]
  },
  {
   "cell_type": "markdown",
   "metadata": {},
   "source": [
    "<hr>\n",
    "\n",
    "### Q1. Find the value of T(2), given that `T(0)=5` for the recurrence relation \n",
    "### &emsp;&emsp;&emsp;&emsp;&emsp;&emsp;&emsp;&emsp;&emsp;&emsp;&emsp; `T(n) = 3T(n-1) + 12n`.\n",
    "\n",
    "### Sol: \n",
    "1. Substituting `n = 1` in `T(n) = 3T(n-1) + 12n`\n",
    "\n",
    "&emsp;&emsp;&emsp;&emsp;&emsp;&emsp;&emsp;&emsp;&emsp;&emsp;&emsp;&emsp;&emsp;&emsp;&emsp;&emsp;&emsp;&emsp;$\\mathrm{\\Rightarrow \\boldsymbol{T(\\textcolor{green}{1})} = 3T(\\textcolor{green}{1} -1) + 12 \\times \\textcolor{green}{1}}$\n",
    "\n",
    "&emsp;&emsp;&emsp;&emsp;&emsp;&emsp;&emsp;&emsp;&emsp;&emsp;&emsp;&emsp;&emsp;&emsp;&emsp;&emsp;&emsp;&emsp;$\\mathrm{\\Rightarrow \\boldsymbol{T(1)} = 3T(0) + 12}$\n",
    "\n",
    "&emsp;&emsp;Given **`T(0) = 5`**\n",
    "\n",
    "&emsp;&emsp;&emsp;&emsp;&emsp;&emsp;&emsp;&emsp;&emsp;&emsp;&emsp;&emsp;&emsp;&emsp;&emsp;&emsp;&emsp;&emsp;$\\mathrm{\\Rightarrow \\boldsymbol{T(1)} = 3 \\times \\textcolor{green}{5} + 12}$\n",
    "\n",
    "&emsp;&emsp;&emsp;&emsp;&emsp;&emsp;&emsp;&emsp;&emsp;&emsp;&emsp;&emsp;&emsp;&emsp;&emsp;&emsp;&emsp;&emsp;$\\mathrm{\\Rightarrow \\boldsymbol{T(1)} = \\textcolor{green}{15} + 12}$\n",
    "\n",
    "&emsp;&emsp;&emsp;&emsp;&emsp;&emsp;&emsp;&emsp;&emsp;&emsp;&emsp;&emsp;&emsp;&emsp;&emsp;&emsp;&emsp;&emsp;$\\mathrm{\\implies \\boxed{\\boldsymbol{T(1)} = \\textcolor{green}{27}}}$\n",
    "\n",
    "2. Now substituting `n = 2` in `T(n) = 3T(n-1) + 12n`\n",
    "\n",
    "&emsp;&emsp;&emsp;&emsp;&emsp;&emsp;&emsp;&emsp;&emsp;&emsp;&emsp;&emsp;&emsp;&emsp;&emsp;&emsp;&emsp;&emsp;$\\mathrm{\\Rightarrow \\boldsymbol{T(\\textcolor{green}{2})} = 3T(\\textcolor{green}{2} -1) + 12 \\times \\textcolor{green}{2}}$\n",
    "\n",
    "&emsp;&emsp;&emsp;&emsp;&emsp;&emsp;&emsp;&emsp;&emsp;&emsp;&emsp;&emsp;&emsp;&emsp;&emsp;&emsp;&emsp;&emsp;$\\mathrm{\\Rightarrow \\boldsymbol{T(2)} = 3T\\color{green}{(1)}+ 24}$\n",
    "\n",
    "&emsp;&emsp;Substituting, **`T(1) = 27`**\n",
    "\n",
    "&emsp;&emsp;&emsp;&emsp;&emsp;&emsp;&emsp;&emsp;&emsp;&emsp;&emsp;&emsp;&emsp;&emsp;&emsp;&emsp;&emsp;&emsp;$\\mathrm{\\Rightarrow \\boldsymbol{T(2)} = 3 \\times \\textcolor{green}{27}  + 24}$\n",
    "\n",
    "&emsp;&emsp;&emsp;&emsp;&emsp;&emsp;&emsp;&emsp;&emsp;&emsp;&emsp;&emsp;&emsp;&emsp;&emsp;&emsp;&emsp;&emsp;$\\mathrm{\\Rightarrow\\boldsymbol{T(2)} = \\textcolor{green}{81}  + 24}$\n",
    "\n",
    "&emsp;&emsp;&emsp;&emsp;&emsp;&emsp;&emsp;&emsp;&emsp;&emsp;&emsp;&emsp;&emsp;&emsp;&emsp;&emsp;&emsp;&emsp;$\\mathrm{\\implies \\color{green}{\\boxed{\\boldsymbol{T(2)} = \\textcolor{green}{105}}}}$"
   ]
  },
  {
   "cell_type": "markdown",
   "metadata": {},
   "source": [
    "<hr>\n",
    "\n",
    "### Q2. Given a recurrence relation, solve it using the substitution method:\n",
    "\n",
    "#### a.&emsp;&emsp;&emsp;&emsp;&emsp;&emsp;&emsp;&emsp;&emsp;&emsp;&emsp;`T(n) = T(n-1) + c`\n",
    "\n",
    "### Sol:\n",
    "&emsp;&emsp;&emsp;&emsp;&emsp;&emsp;&emsp;&emsp;&emsp;&emsp;&emsp;&emsp;&emsp;&emsp;&emsp;&emsp;&emsp;&emsp;&emsp;&emsp;$\\mathrm{\\boxed{\\boldsymbol{T(n)} = T(n-1) + c}} \\;\\rightarrow eqn1$\n",
    "\n",
    "1. Substituting `n = n - 1` in `eqn1`\n",
    "\n",
    "&emsp;&emsp;&emsp;&emsp;&emsp;&emsp;&emsp;&emsp;&emsp;&emsp;&emsp;&emsp;&emsp;&emsp;&emsp;&emsp;&emsp;&emsp;$\\mathrm{\\Rightarrow \\boldsymbol{T(\\textcolor{green}{n - 1})} = T(\\textcolor{green}{(n - 1)} -1) + c}$\n",
    "\n",
    "&emsp;&emsp;&emsp;&emsp;&emsp;&emsp;&emsp;&emsp;&emsp;&emsp;&emsp;&emsp;&emsp;&emsp;&emsp;&emsp;&emsp;&emsp;$\\mathrm{\\Rightarrow \\color{green}{\\boxed{\\boldsymbol{T(n - 1)} = T(n -2) + c}}} \\;\\rightarrow eqn2$\n",
    "\n",
    "2. Substituting the value of `T(n-1)` from `eqn2` in `eqn1`\n",
    "\n",
    "&emsp;&emsp;&emsp;&emsp;&emsp;&emsp;&emsp;&emsp;&emsp;&emsp;&emsp;&emsp;&emsp;&emsp;&emsp;&emsp;&emsp;&emsp;$\\mathrm{\\Rightarrow \\boldsymbol{T(n)} = [\\; T(\\textcolor{green}{(n - 2)}) + c\\;] + c}$\n",
    "\n",
    "&emsp;&emsp;&emsp;&emsp;&emsp;&emsp;&emsp;&emsp;&emsp;&emsp;&emsp;&emsp;&emsp;&emsp;&emsp;&emsp;&emsp;&emsp;$\\mathrm{\\Rightarrow \\color{green}{\\boxed{\\boldsymbol{T(n)} = T(n -2) + 2c}}} \\;\\rightarrow eqn3$\n",
    "\n",
    "3. Substituting `n = n - 2` in `eqn1`\n",
    "\n",
    "&emsp;&emsp;&emsp;&emsp;&emsp;&emsp;&emsp;&emsp;&emsp;&emsp;&emsp;&emsp;&emsp;&emsp;&emsp;&emsp;&emsp;&emsp;$\\mathrm{\\Rightarrow \\boldsymbol{T(\\textcolor{green}{n - 2})} = T(\\textcolor{green}{(n - 2)} -1) + c}$\n",
    "\n",
    "&emsp;&emsp;&emsp;&emsp;&emsp;&emsp;&emsp;&emsp;&emsp;&emsp;&emsp;&emsp;&emsp;&emsp;&emsp;&emsp;&emsp;&emsp;$\\mathrm{\\Rightarrow \\color{green}{\\boxed{\\boldsymbol{T(n - 2)} = T(n -3) + c}}} \\;\\rightarrow eqn4$\n",
    "\n",
    "4. Substituting the value of `T(n-2)` from `eqn4` in `eqn3`\n",
    "\n",
    "&emsp;&emsp;&emsp;&emsp;&emsp;&emsp;&emsp;&emsp;&emsp;&emsp;&emsp;&emsp;&emsp;&emsp;&emsp;&emsp;&emsp;&emsp;$\\mathrm{\\Rightarrow \\boldsymbol{T(n)} = [\\; T(\\textcolor{green}{(n - 3)}) + c\\;] + 2c}$\n",
    "\n",
    "&emsp;&emsp;&emsp;&emsp;&emsp;&emsp;&emsp;&emsp;&emsp;&emsp;&emsp;&emsp;&emsp;&emsp;&emsp;&emsp;&emsp;&emsp;$\\mathrm{\\Rightarrow \\color{green}{\\boxed{\\boldsymbol{T(n)} = T(n -3) + 3c}}} \\;\\rightarrow eqn5$\n",
    "\n",
    "5. Generalising for `k` times we get,\n",
    "\n",
    "&emsp;&emsp;&emsp;&emsp;&emsp;&emsp;&emsp;&emsp;&emsp;&emsp;&emsp;&emsp;&emsp;&emsp;&emsp;&emsp;&emsp;&emsp;$\\mathrm{\\Rightarrow \\color{green}{\\boxed{\\boldsymbol{T(n)} = T(n -k) + k.c}}} \\;\\rightarrow eqn6$\n",
    "\n",
    "6. Substituting `k = n-1` in `eqn6` i.e., repeating the operation `n-1` times, we get \n",
    "\n",
    "&emsp;&emsp;&emsp;&emsp;&emsp;&emsp;&emsp;&emsp;&emsp;&emsp;&emsp;&emsp;&emsp;&emsp;&emsp;&emsp;&emsp;&emsp;$\\mathrm{\\Rightarrow {\\boldsymbol{T(n)} = T(n - \\color{green}{(n-1)}\\color{black}{)} + \\color{green}{(n-1)}.c}}$\n",
    "\n",
    "&emsp;&emsp;&emsp;&emsp;&emsp;&emsp;&emsp;&emsp;&emsp;&emsp;&emsp;&emsp;&emsp;&emsp;&emsp;&emsp;&emsp;&emsp;$\\mathrm{\\implies  \\color{green}{\\boxed{\\boldsymbol{T(n)} = T(1) + (n-1).c}}}$"
   ]
  },
  {
   "cell_type": "markdown",
   "metadata": {},
   "source": [
    "<hr>\n",
    "\n",
    "### b.&emsp;&emsp;&emsp;&emsp;&emsp;&emsp;&emsp;&emsp;&emsp;`T(n) = 2T(n/2) + n`\n",
    "### Sol:\n",
    "&emsp;&emsp;&emsp;&emsp;&emsp;&emsp;&emsp;&emsp;&emsp;&emsp;&emsp;&emsp;&emsp;&emsp;&emsp;&emsp;&emsp;&emsp;&emsp;&emsp;$\\mathrm{\\boxed{\\boldsymbol{T(n)} = 2T\\left(\\frac{n}{2}\\right) + n}} \\;\\rightarrow eqn1$\n",
    "\n",
    "1. Substituting `n = n/2` in `eqn1`\n",
    "\n",
    "&emsp;&emsp;&emsp;&emsp;&emsp;&emsp;&emsp;&emsp;&emsp;&emsp;&emsp;&emsp;&emsp;&emsp;&emsp;&emsp;&emsp;&emsp;$\\mathrm{\\Rightarrow \\boxed{\\boldsymbol{T\\textcolor{green}{\\left(\\frac{n}{2}\\right)}} = 2T\\color{green}{\\left(\\frac{n}{2^2}\\right)}+ \\color{green}{\\left(\\frac{n}{2}\\right)}}}\\;\\rightarrow eqn2$\n",
    "\n",
    "2. Substituting the value of `T(n/2)` from `eqn2` in `eqn1`\n",
    "\n",
    "&emsp;&emsp;&emsp;&emsp;&emsp;&emsp;&emsp;&emsp;&emsp;&emsp;&emsp;&emsp;&emsp;&emsp;&emsp;&emsp;&emsp;&emsp;$\\mathrm{\\Rightarrow \\boldsymbol{T(n)} = 2 \\times[\\; \\color{green}{2T\\left(\\frac{n}{2^2}\\right)+ \\left(\\frac{n}{2}\\right)}}\\;] + n$\n",
    "\n",
    "&emsp;&emsp;&emsp;&emsp;&emsp;&emsp;&emsp;&emsp;&emsp;&emsp;&emsp;&emsp;&emsp;&emsp;&emsp;&emsp;&emsp;&emsp;$\\mathrm{\\Rightarrow \\boldsymbol{T(n)} = 2^2.T\\left(\\frac{n}{2^2}\\right)+ 2.\\left(\\frac{n}{2}\\right) + n}$\n",
    "\n",
    "&emsp;&emsp;&emsp;&emsp;&emsp;&emsp;&emsp;&emsp;&emsp;&emsp;&emsp;&emsp;&emsp;&emsp;&emsp;&emsp;&emsp;&emsp;$\\mathrm{\\Rightarrow \\boxed{\\boldsymbol{T(n)} = 2^2.T\\left(\\frac{n}{2^2}\\right)+ \\color{green}{2n}}}\\;\\rightarrow eqn3$\n",
    "\n",
    "3. Substituting `n = n/4` in `eqn1`\n",
    "\n",
    "&emsp;&emsp;&emsp;&emsp;&emsp;&emsp;&emsp;&emsp;&emsp;&emsp;&emsp;&emsp;&emsp;&emsp;&emsp;&emsp;&emsp;&emsp;$\\mathrm{\\Rightarrow \\boxed{\\boldsymbol{T\\textcolor{green}{\\left(\\frac{n}{2^2}\\right)}} = 2T\\color{green}{\\left(\\frac{n}{2^3}\\right)}+ \\color{green}{\\left(\\frac{n}{2^2}\\right)}}}\\;\\rightarrow eqn4$\n",
    "\n",
    "4. Substituting the value of `T(n/4)` from `eqn4` in `eqn3`\n",
    "\n",
    "&emsp;&emsp;&emsp;&emsp;&emsp;&emsp;&emsp;&emsp;&emsp;&emsp;&emsp;&emsp;&emsp;&emsp;&emsp;&emsp;&emsp;&emsp;$\\mathrm{\\Rightarrow \\boldsymbol{T(n)} = 2^2\\times[\\; \\color{green}{2T\\left(\\frac{n}{2^3}\\right)+ \\left(\\frac{n}{2^2}\\right)}}\\;] + 2n$\n",
    "\n",
    "&emsp;&emsp;&emsp;&emsp;&emsp;&emsp;&emsp;&emsp;&emsp;&emsp;&emsp;&emsp;&emsp;&emsp;&emsp;&emsp;&emsp;&emsp;$\\mathrm{\\Rightarrow \\boldsymbol{T(n)} = 2^3.T\\left(\\frac{n}{2^3}\\right)+ 2^2.\\left(\\frac{n}{2^2}\\right) + 2n}$\n",
    "\n",
    "&emsp;&emsp;&emsp;&emsp;&emsp;&emsp;&emsp;&emsp;&emsp;&emsp;&emsp;&emsp;&emsp;&emsp;&emsp;&emsp;&emsp;&emsp;$\\mathrm{\\Rightarrow \\boxed{\\boldsymbol{T(n)} = 2^3.T\\left(\\frac{n}{2^3}\\right)+ \\color{green}{3n}}}\\;\\rightarrow eqn5$\n",
    "\n",
    "5. Generalising for `k` times we get,\n",
    "\n",
    "&emsp;&emsp;&emsp;&emsp;&emsp;&emsp;&emsp;&emsp;&emsp;&emsp;&emsp;&emsp;&emsp;&emsp;&emsp;&emsp;&emsp;&emsp;$\\mathrm{\\Rightarrow \\color{green}{\\boxed{\\boldsymbol{T(n)} = 2^k.T\\left(\\frac{n}{2^k}\\right)+ k.n}}}\\;\\rightarrow eqn6$\n",
    "\n",
    "6. Substituting $\\mathrm{\\left(\\frac{n}{2^k}\\right) = 1, \\; \\text{i.e.,}\\; 2^k = n \\implies \\boxed{k = \\log_2n}}$ in `eqn6`\n",
    "\n",
    "&emsp;&emsp;&emsp;&emsp;&emsp;&emsp;&emsp;&emsp;&emsp;&emsp;&emsp;&emsp;&emsp;&emsp;&emsp;&emsp;&emsp;&emsp;$\\mathrm{\\Rightarrow \\boldsymbol{T(n)} = 2^{\\color{green}{\\log_2{n}}}.T\\left(\\frac{n}{2^{\\color{green}{\\log_2{n}}}}\\right)+ ({\\color{green}{\\log_2{n}}})n}$\n",
    "\n",
    "&emsp;&emsp;&emsp;&emsp;&emsp;&emsp;&emsp;&emsp;&emsp;&emsp;&emsp;&emsp;&emsp;&emsp;&emsp;&emsp;&emsp;&emsp;$\\mathrm{\\Rightarrow \\boldsymbol{T(n)} = {\\color{green}{n}}.T\\left(\\frac{n}{{\\color{green}{n}}}\\right)+ n.{\\log_2{n}}}$\n",
    "\n",
    "&emsp;&emsp;&emsp;&emsp;&emsp;&emsp;&emsp;&emsp;&emsp;&emsp;&emsp;&emsp;&emsp;&emsp;&emsp;&emsp;&emsp;&emsp;$\\mathrm{\\implies {\\color{green}{\\boxed{\\boldsymbol{T(n)} = n.T(1)+ n.{\\log_2{n}}}}}}$"
   ]
  },
  {
   "cell_type": "markdown",
   "metadata": {},
   "source": [
    "<hr>\n",
    "\n",
    "### c.&emsp;&emsp;&emsp;&emsp;&emsp;&emsp;&emsp;&emsp;&emsp;`T(n) = 2T(n/2) + c`\n",
    "### Sol:\n",
    "&emsp;&emsp;&emsp;&emsp;&emsp;&emsp;&emsp;&emsp;&emsp;&emsp;&emsp;&emsp;&emsp;&emsp;&emsp;&emsp;&emsp;&emsp;&emsp;&emsp;$\\mathrm{\\boxed{\\boldsymbol{T(n)} = 2T\\left(\\frac{n}{2}\\right) + c}} \\;\\rightarrow eqn1$\n",
    "\n",
    "1. Substituting `n=n/2`​ in `eqn1`\n",
    "\n",
    "&emsp;&emsp;&emsp;&emsp;&emsp;&emsp;&emsp;&emsp;&emsp;&emsp;&emsp;&emsp;&emsp;&emsp;&emsp;&emsp;&emsp;&emsp;$\\mathrm{\\Rightarrow \\boxed{\\boldsymbol{T\\textcolor{green}{\\left(\\frac{n}{2}\\right)}} = 2T{\\color{green}{\\left(\\frac{n}{2^2}\\right)}}+ c}}\\;\\rightarrow eqn2$\n",
    "\n",
    "2. Substituting the value of `T(n/2)` from `eqn2` in `eqn1`\n",
    "\n",
    "&emsp;&emsp;&emsp;&emsp;&emsp;&emsp;&emsp;&emsp;&emsp;&emsp;&emsp;&emsp;&emsp;&emsp;&emsp;&emsp;&emsp;&emsp;$\\mathrm{\\Rightarrow \\boldsymbol{T(n)} = 2 \\times[\\; \\color{green}{2T\\left(\\frac{n}{2^2}\\right)+ c}}\\;] + c$\n",
    "\n",
    "&emsp;&emsp;&emsp;&emsp;&emsp;&emsp;&emsp;&emsp;&emsp;&emsp;&emsp;&emsp;&emsp;&emsp;&emsp;&emsp;&emsp;&emsp;$\\mathrm{\\Rightarrow \\boldsymbol{T(n)} = 2^2.T\\left(\\frac{n}{2^2}\\right)+ 2c + c}$\n",
    "\n",
    "&emsp;&emsp;&emsp;&emsp;&emsp;&emsp;&emsp;&emsp;&emsp;&emsp;&emsp;&emsp;&emsp;&emsp;&emsp;&emsp;&emsp;&emsp;$\\mathrm{\\Rightarrow \\boxed{\\boldsymbol{T(n)} = 2^2.T\\left(\\frac{n}{2^2}\\right)+ \\color{green}{3c}}}\\;\\rightarrow eqn3$\n",
    "\n",
    "3. Substituting `n = n/4` in `eqn1`\n",
    "\n",
    "&emsp;&emsp;&emsp;&emsp;&emsp;&emsp;&emsp;&emsp;&emsp;&emsp;&emsp;&emsp;&emsp;&emsp;&emsp;&emsp;&emsp;&emsp;$\\mathrm{\\Rightarrow \\boxed{\\boldsymbol{T\\textcolor{green}{\\left(\\frac{n}{2^2}\\right)}} = 2T{\\color{green}{\\left(\\frac{n}{2^3}\\right)}}+ c}}\\;\\rightarrow eqn4$\n",
    "\n",
    "4. Substituting the value of `T(n/4)` from `eqn4` in `eqn3`\n",
    "\n",
    "&emsp;&emsp;&emsp;&emsp;&emsp;&emsp;&emsp;&emsp;&emsp;&emsp;&emsp;&emsp;&emsp;&emsp;&emsp;&emsp;&emsp;&emsp;$\\mathrm{\\Rightarrow \\boldsymbol{T(n)} = 2^2\\times[\\; {\\color{green}{2T\\left(\\frac{n}{2^3}\\right)+ c}}\\;] + 3c}$\n",
    "\n",
    "&emsp;&emsp;&emsp;&emsp;&emsp;&emsp;&emsp;&emsp;&emsp;&emsp;&emsp;&emsp;&emsp;&emsp;&emsp;&emsp;&emsp;&emsp;$\\mathrm{\\Rightarrow \\boldsymbol{T(n)} = 2^3.T\\left(\\frac{n}{2^3}\\right)+ {\\color{green}{4c}} + 3c}$\n",
    "\n",
    "&emsp;&emsp;&emsp;&emsp;&emsp;&emsp;&emsp;&emsp;&emsp;&emsp;&emsp;&emsp;&emsp;&emsp;&emsp;&emsp;&emsp;&emsp;$\\mathrm{\\Rightarrow \\boxed{\\boldsymbol{T(n)} = 2^3.T\\left(\\frac{n}{2^3}\\right)+ \\color{green}{7c}}}\\;\\rightarrow eqn5$\n",
    "\n",
    "5. Generalising for `k` times we get,\n",
    "\n",
    "&emsp;&emsp;&emsp;&emsp;&emsp;&emsp;&emsp;&emsp;&emsp;&emsp;&emsp;&emsp;&emsp;&emsp;&emsp;&emsp;&emsp;&emsp;$\\mathrm{\\Rightarrow \\color{green}{\\boxed{\\boldsymbol{T(n)} = 2^k.T\\left(\\frac{n}{2^k}\\right)+ (2^k-1)c}}}\\;\\rightarrow eqn6$\n",
    "\n",
    "6. Substituting $\\mathrm{\\left(\\frac{n}{2^k}\\right) = 1, \\; \\text{i.e.,}\\; 2^k = n \\implies \\boxed{k = \\log_2n}}$ in `eqn6`\n",
    "\n",
    "&emsp;&emsp;&emsp;&emsp;&emsp;&emsp;&emsp;&emsp;&emsp;&emsp;&emsp;&emsp;&emsp;&emsp;&emsp;&emsp;&emsp;&emsp;$\\mathrm{\\Rightarrow \\boldsymbol{T(n)} = 2^{\\color{green}{\\log_2{n}}}.T\\left(\\frac{n}{2^{\\color{green}{\\log_2{n}}}}\\right)+ (2^{\\color{green}{{\\log_2{n}}}}-1)c}$\n",
    "\n",
    "&emsp;&emsp;&emsp;&emsp;&emsp;&emsp;&emsp;&emsp;&emsp;&emsp;&emsp;&emsp;&emsp;&emsp;&emsp;&emsp;&emsp;&emsp;$\\mathrm{\\Rightarrow \\boldsymbol{T(n)} = {\\color{green}{n}}.T\\left(\\frac{n}{{\\color{green}{n}}}\\right)+ ({\\color{green}{n}}-1)c}$\n",
    "\n",
    "&emsp;&emsp;&emsp;&emsp;&emsp;&emsp;&emsp;&emsp;&emsp;&emsp;&emsp;&emsp;&emsp;&emsp;&emsp;&emsp;&emsp;&emsp;$\\mathrm{\\implies {\\color{green}{\\boxed{\\boldsymbol{T(n)} = n.T(1)+ (n-1)c}}}}$"
   ]
  },
  {
   "cell_type": "markdown",
   "metadata": {},
   "source": [
    "<hr>\n",
    "\n",
    "### d.&emsp;&emsp;&emsp;&emsp;&emsp;&emsp;&emsp;&emsp;&emsp;`T(n) = T(n/2) + c`\n",
    "### Sol:\n",
    "&emsp;&emsp;&emsp;&emsp;&emsp;&emsp;&emsp;&emsp;&emsp;&emsp;&emsp;&emsp;&emsp;&emsp;&emsp;&emsp;&emsp;&emsp;&emsp;&emsp;$\\mathrm{\\boxed{\\boldsymbol{T(n)} = T\\left(\\frac{n}{2}\\right) + c}} \\;\\rightarrow eqn1$\n",
    "\n",
    "1. Substituting `n=n/2`​ in `eqn1`\n",
    "\n",
    "&emsp;&emsp;&emsp;&emsp;&emsp;&emsp;&emsp;&emsp;&emsp;&emsp;&emsp;&emsp;&emsp;&emsp;&emsp;&emsp;&emsp;&emsp;$\\mathrm{\\Rightarrow \\boxed{\\boldsymbol{T\\textcolor{green}{\\left(\\frac{n}{2}\\right)}} = T{\\color{green}{\\left(\\frac{n}{2^2}\\right)}}+ c}}\\;\\rightarrow eqn2$\n",
    "\n",
    "2. Substituting the value of `T(n/2)` from `eqn2` in `eqn1`\n",
    "\n",
    "&emsp;&emsp;&emsp;&emsp;&emsp;&emsp;&emsp;&emsp;&emsp;&emsp;&emsp;&emsp;&emsp;&emsp;&emsp;&emsp;&emsp;&emsp;$\\mathrm{\\Rightarrow \\boldsymbol{T(n)} = [\\; \\color{green}{T\\left(\\frac{n}{2^2}\\right)+ c}}\\;] + c$\n",
    "\n",
    "&emsp;&emsp;&emsp;&emsp;&emsp;&emsp;&emsp;&emsp;&emsp;&emsp;&emsp;&emsp;&emsp;&emsp;&emsp;&emsp;&emsp;&emsp;$\\mathrm{\\Rightarrow \\boldsymbol{T(n)} = T\\left(\\frac{n}{2^2}\\right)+ c + c}$\n",
    "\n",
    "&emsp;&emsp;&emsp;&emsp;&emsp;&emsp;&emsp;&emsp;&emsp;&emsp;&emsp;&emsp;&emsp;&emsp;&emsp;&emsp;&emsp;&emsp;$\\mathrm{\\Rightarrow \\boxed{\\boldsymbol{T(n)} = T\\left(\\frac{n}{2^2}\\right)+ \\color{green}{2c}}}\\;\\rightarrow eqn3$\n",
    "\n",
    "3. Substituting `n = n/4` in `eqn1`\n",
    "\n",
    "&emsp;&emsp;&emsp;&emsp;&emsp;&emsp;&emsp;&emsp;&emsp;&emsp;&emsp;&emsp;&emsp;&emsp;&emsp;&emsp;&emsp;&emsp;$\\mathrm{\\Rightarrow \\boxed{\\boldsymbol{T\\textcolor{green}{\\left(\\frac{n}{2^2}\\right)}} = T{\\color{green}{\\left(\\frac{n}{2^3}\\right)}}+ c}}\\;\\rightarrow eqn4$\n",
    "\n",
    "4. Substituting the value of `T(n/4)` from `eqn4` in `eqn3`\n",
    "\n",
    "&emsp;&emsp;&emsp;&emsp;&emsp;&emsp;&emsp;&emsp;&emsp;&emsp;&emsp;&emsp;&emsp;&emsp;&emsp;&emsp;&emsp;&emsp;$\\mathrm{\\Rightarrow \\boldsymbol{T(n)} = [\\; {\\color{green}{T\\left(\\frac{n}{2^3}\\right)+ c}}\\;] + 2c}$\n",
    "\n",
    "&emsp;&emsp;&emsp;&emsp;&emsp;&emsp;&emsp;&emsp;&emsp;&emsp;&emsp;&emsp;&emsp;&emsp;&emsp;&emsp;&emsp;&emsp;$\\mathrm{\\Rightarrow \\boxed{\\boldsymbol{T(n)} = T\\left(\\frac{n}{2^3}\\right)+ \\color{green}{3c}}}\\;\\rightarrow eqn5$\n",
    "\n",
    "5. Generalising for `k` times we get,\n",
    "\n",
    "&emsp;&emsp;&emsp;&emsp;&emsp;&emsp;&emsp;&emsp;&emsp;&emsp;&emsp;&emsp;&emsp;&emsp;&emsp;&emsp;&emsp;&emsp;$\\mathrm{\\Rightarrow \\color{green}{\\boxed{\\boldsymbol{T(n)} = T\\left(\\frac{n}{2^k}\\right)+ k.c}}}\\;\\rightarrow eqn6$\n",
    "\n",
    "6. Substituting $\\mathrm{\\left(\\frac{n}{2^k}\\right) = 1, \\; \\text{i.e.,}\\; 2^k = n \\implies \\boxed{k = \\log_2n}}$ in `eqn6`\n",
    "\n",
    "&emsp;&emsp;&emsp;&emsp;&emsp;&emsp;&emsp;&emsp;&emsp;&emsp;&emsp;&emsp;&emsp;&emsp;&emsp;&emsp;&emsp;&emsp;$\\mathrm{\\Rightarrow \\boldsymbol{T(n)} = T\\left(\\frac{n}{2^{\\color{green}{\\log_2{n}}}}\\right)+ ({\\color{green}{{\\log_2{n}}}})c}$\n",
    "\n",
    "&emsp;&emsp;&emsp;&emsp;&emsp;&emsp;&emsp;&emsp;&emsp;&emsp;&emsp;&emsp;&emsp;&emsp;&emsp;&emsp;&emsp;&emsp;$\\mathrm{\\Rightarrow \\boldsymbol{T(n)} = T\\left(\\frac{n}{{\\color{green}{n}}}\\right)+ c.\\log_2{n}}$\n",
    "\n",
    "&emsp;&emsp;&emsp;&emsp;&emsp;&emsp;&emsp;&emsp;&emsp;&emsp;&emsp;&emsp;&emsp;&emsp;&emsp;&emsp;&emsp;&emsp;$\\mathrm{\\implies {\\color{green}{\\boxed{\\boldsymbol{T(n)} = T(1)+ c.\\log_2{n}}}}}$"
   ]
  },
  {
   "cell_type": "markdown",
   "metadata": {},
   "source": [
    "<hr>"
   ]
  },
  {
   "cell_type": "markdown",
   "metadata": {},
   "source": [
    "<hr>\n",
    "\n",
    "### Q3. Given a recurrence relation, solve it using the recursive tree approach:\n",
    "\n",
    "### a.&emsp;&emsp;&emsp;&emsp;&emsp;&emsp;&emsp;&emsp;&emsp;`T(n) = 2T(n-1) +1`\n"
   ]
  },
  {
   "cell_type": "markdown",
   "metadata": {},
   "source": [
    "<hr>\n",
    "\n",
    "### b.&emsp;&emsp;&emsp;&emsp;&emsp;&emsp;&emsp;&emsp;&emsp;`T(n) = 2T(n/2) + n`"
   ]
  },
  {
   "cell_type": "markdown",
   "metadata": {},
   "source": [
    "- $\\implies$\n",
    "- $\\sin$\n",
    "- $\\color{red}hello$ there$\n",
    "- $\\mathrm{\\implies \\boldsymbol{T} = 2T(n-1) + 1}$\n",
    "- $\\sum$\n",
    "- $\\bigcirc{1}$\n",
    "- $2^{\\log_2{n}}$"
   ]
  },
  {
   "cell_type": "markdown",
   "metadata": {},
   "source": [
    "Sol:\n",
    "\n",
    "                    $\\mathrm{\\boxed{\\boldsymbol{T(n)} = 2T\\left(\\frac{n}{2}\\right) + c}} ;\\rightarrow eqn1$\n",
    "\n",
    "    Substituting n=n2n=2n​ in eqn1eqn1:\n",
    "\n",
    "                 $\\mathrm{\\Rightarrow \\boxed{\\boldsymbol{T\\left(\\frac{n}{2}\\right)} = 2T\\left(\\frac{n}{2^2}\\right)+ c}};\\rightarrow eqn2$\n",
    "\n",
    "    Substituting the value of T(n2)T(2n​) from eqn2eqn2 in eqn1eqn1:\n",
    "\n",
    "                 $\\mathrm{\\Rightarrow \\boldsymbol{T(n)} = 2 \\times[\\; 2T\\left(\\frac{n}{2^2}\\right)+ c}\\;] + c$\n",
    "\n",
    "                 $\\mathrm{\\Rightarrow \\boldsymbol{T(n)} = 2^2.T\\left(\\frac{n}{2^2}\\right)+ 2c + c}$\n",
    "\n",
    "                 $\\mathrm{\\Rightarrow \\boxed{\\boldsymbol{T(n)} = 2^2.T\\left(\\frac{n}{2^2}\\right)+ \\color{green}{3c}}};\\rightarrow eqn3$\n",
    "\n",
    "    Substituting n=n4n=4n​ in eqn1eqn1:\n",
    "\n",
    "                 $\\mathrm{\\Rightarrow \\boxed{\\boldsymbol{T\\left(\\frac{n}{2^2}\\right)} = 2T\\left(\\frac{n}{2^3}\\right)+ c}};\\rightarrow eqn4$\n",
    "\n",
    "    Substituting the value of T(n22)T(22n​) from eqn4eqn4 in eqn3eqn3:\n",
    "\n",
    "                 $\\mathrm{\\Rightarrow \\boldsymbol{T(n)} = 2^2\\times[; 2T\\left(\\frac{n}{2^3}\\right)+ c}; + 3c$\n",
    "\n",
    "                 $\\mathrm{\\Rightarrow \\boldsymbol{T(n)} = 2^3.T\\left(\\frac{n}{2^3}\\right)+ 2^2c + 3c}$\n",
    "\n",
    "                 $\\mathrm{\\Rightarrow \\boxed{\\boldsymbol{T(n)} = 2^3.T\\left(\\frac{n}{2^3}\\right)+ \\color{green}{7c}}};\\rightarrow eqn5$\n",
    "\n",
    "    Generalising for kk times we get,\n",
    "\n",
    "                  $\\mathrm{\\Rightarrow \\color{green}{\\boxed{\\boldsymbol{T(n)} = 2^k.T\\left(\\frac{n}{2^k}\\right)+ kc}}};\\rightarrow eqn6$\n",
    "\n",
    "    Substituting n2k=12kn​=1 (i.e., 2k=n2k=n implies k=log⁡2nk=log2​n) in eqn6eqn6:\n",
    "\n",
    "                  $\\mathrm{\\Rightarrow \\boldsymbol{T(n)} = 2^{\\color{green}{\\log_2n}}.T\\left(\\frac{n}{2^{\\color{green}{\\log_2n}}}\\right)+ {\\color{green}{\\log_2n}}c}$\n",
    "\n",
    "                  $\\mathrm{\\Rightarrow \\boldsymbol{T(n)} = {\\color{green}{n}}.T\\left(\\frac{n}{{\\color{green}{n}}}\\right)+ {\\color{green}{n}}c}$\n",
    "\n",
    "                  $\\mathrm{\\implies {\\color{green}{\\boxed{\\boldsymbol{T(n)} = n[T(1)+c]}}}}$"
   ]
  }
 ],
 "metadata": {
  "language_info": {
   "name": "python"
  }
 },
 "nbformat": 4,
 "nbformat_minor": 2
}
